Going deeper in susbtitution elim raises need for more inversions

formalization/substitution_elim.v
@@ -1,8 +1,13 @@
 Require Import syntax.
 Require ett ptt.
+Require Import ptt_inversion.
+Require ptt_sanity.
+Require Import tactics.
 
 Inductive subst_free_term : term -> Type :=
-  | subst_free_var : forall n, subst_free_term (var n)
+  | subst_free_var :
+      forall n,
+        subst_free_term (var n)
 
   | subst_free_lam :
       forall A B u,
@@ -18,24 +23,74 @@ Inductive subst_free_term : term -> Type :=
         subst_free_type B ->
         subst_free_term v ->
         subst_free_term (app u A B v)
-(*
-  | subst_free_refl : type -> term -> term
-  | subst_free_j : type -> term -> type -> term -> term -> term -> term
+
+  | subst_free_refl :
+      forall A u,
+        subst_free_type A ->
+        subst_free_term u ->
+        subst_free_term (refl A u)
+
+  | subst_free_j :
+      forall A u C w v p,
+        subst_free_type A ->
+        subst_free_term u ->
+        subst_free_type C ->
+        subst_free_term w ->
+        subst_free_term v ->
+        subst_free_term p ->
+        subst_free_term (j A u C w v p)
+
   (* NB: subst is not subst free! *)
-  | subst_free_exfalso : type -> term -> term
-  | subst_free_unit : term
-  | subst_free_true : term
-  | subst_free_false : term
-  | subst_free_cond : type -> term -> term -> term -> term
-*)
+
+  | subst_free_exfalso :
+      forall A u,
+        subst_free_type A ->
+        subst_free_term u ->
+        subst_free_term (exfalso A u)
+
+  | subst_free_unit :
+      subst_free_term unit
+
+  | subst_free_true :
+      subst_free_term true
+
+  | subst_free_false :
+      subst_free_term false
+
+  | subst_free_cond :
+      forall A u v w,
+        subst_free_type A ->
+        subst_free_term u ->
+        subst_free_term v ->
+        subst_free_term w ->
+        subst_free_term (cond A u v w)
+
 with subst_free_type : type -> Type :=
-(*   | subst_free_Prod : type -> type -> type
-     | subst_free_Id : type -> term -> term -> type
-     | subst_free_Subst : type -> substitution -> type
-     | subst_free_Empty : type
-     | subst_free_Unit : type
-*)
-     | subst_free_Bool : subst_free_type Bool.
+
+  | subst_free_Prod :
+      forall A B,
+        subst_free_type A ->
+        subst_free_type B ->
+        subst_free_type (Prod A B)
+
+  | subst_free_Id :
+      forall A u v,
+        subst_free_type A ->
+        subst_free_term u ->
+        subst_free_term v ->
+        subst_free_type (Id A u v)
+
+  (* NB: Subst is not subst free! *)
+
+  | subst_free_Empty :
+      subst_free_type Empty
+
+  | subst_free_Unit :
+      subst_free_type Unit
+
+  | subst_free_Bool :
+      subst_free_type Bool
+.
 
 Hypothesis temporary : forall {A}, A.
 Ltac todo := exact temporary.
@@ -49,51 +104,65 @@ Fixpoint elim_term u :
 with elim_type A :
   { B : type &
     subst_free_type B *
-    (forall G, ptt.istype G A -> ett.eqtype G A B) }%type.
+    (forall G, ptt.istype G A -> ett.eqtype G A B)
+  }%type.
 
 Proof.
   (* elim_term *)
-  - {
-    destruct u.
+  - { destruct u.
 
-    (* var *)
-    - exists (var n).
-      todo.
+      (* var *)
+      - exists (var n). split.
+        + constructor.
+        + intros G A H.
+          apply ett.EqRefl.
+          hyp.
 
-    (* lam *)
-    - (* destruct (elim_term ) *)
-      (* We need to have elim_type as well *)
-      todo.
+      (* lam *)
+      - { destruct (elim_type t) as [A [sA fA]].
+          destruct (elim_type t0) as [B [sB fB]].
+          destruct (elim_term u) as [v [sv fv]].
+          exists (lam A B v). split.
+          - now constructor.
+          - intros G T h.
+            destruct (ptt_sanity.sane_isterm G (lam t t0 u) T h).
+            eapply ett.EqTyConv.
+            + eapply ett.CongAbs.
+              * apply fA. todo. (* We need another inversion lemma. *)
+              * apply fB. todo.
+              * apply fv. todo.
+            + todo. (* Also part of the inversion lemma. *)
+        }
 
-    (* app *)
-    - todo.
+      (* app *)
+      - todo.
 
-    (* refl *)
-    - todo.
+      (* refl *)
+      - todo.
 
-    (* j *)
-    - todo.
+      (* j *)
+      - todo.
 
-    (* subst *)
-    - (* What would we do here? Go though another destruction of u?
+      (* subst *)
+      - (* What would we do here? Go though another destruction of u?
          When does it end? *)
-      todo.
+        todo.
 
-    (* exfalso *)
-    - todo.
+      (* exfalso *)
+      - todo.
 
-    (* unit *)
-    - exists unit. todo.
+      (* unit *)
+      - exists unit. todo.
 
-    (* true *)
-    - exists true. todo.
+      (* true *)
+      - exists true. todo.
 
-    (* false *)
-    - exists false. todo.
+      (* false *)
+      - exists false. todo.
 
-    (* cond *)
-    - todo.
-  }
+      (* cond *)
+      - todo.
+    }
 
   (* elim_type *)
   - { todo. }
